src/Blocking.v
@@ -1,3 +1,5 @@
+Require Import List.
+
 Require Import Common.
 Require Import Syntax Semantics StepDet.
 
@@ -22,11 +24,10 @@ Definition Blocked (msgs: MessagePool TMsg) :=
     InMP m1 msgs -> InMP m2 msgs ->
     tmsg_info m1 = Some ti1 ->
     tmsg_info m2 = Some ti2 ->
-    mid_addr (msg_id (tinfo_rqin ti1)) = mid_addr (msg_id (tinfo_rqin ti2)) ->
+    map (fun msg => mid_addr (msg_id msg)) (tinfo_rqin ti1) =
+    map (fun msg => mid_addr (msg_id msg)) (tinfo_rqin ti2) ->
     ti1 = ti2.
 
 Definition BlockedInv (tst: TState) :=
   Blocked (tst_msgs tst).
-
-Require Import TrsSim.
 
